src/nsearch.v
@@ -1,0 +1,189 @@
+From mathcomp Require Import ssreflect ssrbool ssrfun.
+From mathcomp Require Import ssrnat seq eqtype order.
+From ipcssr Require Import prelude avlmap forms normal_forms kripke_trees in_ngamma
+                           catrev disjunct
+                           le_ks lt_ks nweight nrules.
+
+Section NSearch.
+Context {disp : unit} {A : orderType disp}.
+
+Definition nsearch_invariant (n : nat) :=
+  forall (goal : A) (work : seq (normal_form A)) (ds : seq (disj A))
+         (ni : seq (nested_imp A)) (ai : atomic_imps A) (a : atoms A)
+         (ctx : seq (form A)),
+  invariant a ->
+  invariant ai ->
+  (nweight_Sequent work ds ni ai < n)%N ->
+  regular ai ->
+  a_ai_disj a ai ->
+  a_goal_disj a goal ->
+  nsearch_spec goal work ds ni ai a ctx.
+
+Lemma nsearch_aux n : nsearch_invariant n.
+Proof.
+rewrite /nsearch_invariant; elim: n=>// n IHn goal work ds ni ai a ctx.
+(* 0 < n *)
+rewrite ltnS; elim: work ds ni ai a.
+- (* work = [::] *)
+  case=>[|[i j] ds] ni ai a Ha Hai L R D G.
+  - (* ds = [::] *)
+    move: L; apply: (@lt_ks_rec _ _ (fun ni => (_ <= _)%N -> _) _ ni).
+    case=>/=; first by move=>*; apply: fail.
+    case=>[[a0 a1 n2]|x2 k2] ni2 dni IHl L.
+    - apply: left_nimp.
+      - move=>ni1 L1; case H: (lookup a a1)=>[[]|].
+        - by apply/nax/In_Atoms/optP; exists tt.
+        apply/IHn=>//; last by apply/negOptP.
+        rewrite -(@nweight_sequent_nimp_left _ _ _ _ _ _ _ ni2 _ dni) //.
+        by apply: le_eqv.
+      - move=>ni1 L1.
+        apply: IHn=>//.
+        rewrite (@nweight_sequent_nimp_right _ _ _ _ _ _ _ _ ni1) in L.
+        - by apply/ltn_trans/L.
+        by apply: ge_eqv.
+      move=>/= ni1 k L1.
+      apply: (IHl ni1 [::])=>/=.
+      - by apply: (lt_ks_shift_nd _ _ _ _ _ k).
+      rewrite (nweight_sequent_eqv _ _ _ (catrev_d dni (Undecorated (NImp a0 a1 n2) :: ni2))) //.
+      apply: eqv_ni_trans; first by apply/le_eqv/L1.
+      apply: le_eqv; rewrite !rev_app_app.
+      by apply: le_ni_app_dn=>//; apply: le_ni_refl.
+    apply: shift_ni_dni; apply: IHl=>//.
+    by apply: lt_ks_shift_dd.
+  (* ds=(i,j)::ds) *)
+  apply: left_disj=>ni0 L0; apply: IHn=>//.
+  - rewrite -(@nweight_sequent_left_disj_left _ _ _ j _ _ ni) //.
+    by apply: le_eqv.
+  rewrite -(@nweight_sequent_left_disj_right _ _ i _ _ _ ni) //.
+  by rewrite eqv_ni_sym.
+(* work = _ :: _ *)
+move=>+ work IHw ds ni ai a Ha Hai + R D G; case.
+- (* a = NFalsum *)
+  by move=>L; apply: nefq.
+- (* a = NAtom i *)
+  move=>i L.
+  case: (eqVneq goal i)=>[<-|N].
+  - by apply/nax/in_ngamma_cons_work_head.
+  set aot := (update_atoms i a).
+  case La: aot=>[a' ot]; move: La.
+  rewrite (surjective_pairing aot); case=>_.
+  rewrite lookup_upsert //; case: ot=>[[]|] La.
+  - apply: contradiction_atoms=>//; first by apply/optP; exists tt.
+    by apply: IHw.
+  case Lai: (delete i ai)=>[ai' obs]; move: Lai.
+  rewrite (surjective_pairing (delete _ _)); case=>_.
+  rewrite lookup_delete //; case: obs=>[bs|] Lai.
+  - apply: (left_p_imp_ai _ _ _ _ _ bs)=>//.
+    apply: IHn.
+    - by apply: invariant_upsert.
+    - by apply: invariant_delete.
+    - apply: (leq_trans (n:=nweight_Sequent work ds ni ai)).
+      - by apply: nweight_shift_ai_work.
+      by apply/leq_trans/L.
+    - by apply: regular_del.
+    - by apply: disjs_delete_ai.
+    by apply: goal_disj_insert_a.
+  apply: rule_shift_work_a=>//.
+  apply: IHw=>//.
+  - by apply: invariant_upsert.
+  - by apply: disjs_insert_a=>//; apply/negOptP.
+  by apply: goal_disj_insert_a.
+- (* a = OrF (Atom i) (Atom j) *)
+  move=>i j L.
+  apply/rule_shift_work_ds/IHw=>//.
+  by rewrite -nweight_shift_work_ds.
+- (* a = AImp i b *)
+  move=>i b L.
+  case La : (lookup a i)=>[[]|].
+  - apply: left_p_imp_work; first by apply/optP; exists tt.
+    by apply: IHn.
+  apply: rule_shift_work_ai=>//.
+  apply: IHw=>//.
+  - by apply: invariant_upsert.
+  - by rewrite -nweight_shift_work_ai.
+  - by apply: regular_ins.
+  by apply: disjs_insert_ai=>//; apply/negOptP.
+(* a = NImp x *)
+move=>x L.
+apply/rule_shift_work_ni0/IHw=>//.
+by rewrite -nweight_shift_work_ni0.
+Qed.
+
+(*
+Theorem nsearch :
+ forall (goal : Int) (work : nf_list) (ctx : flist),
+ (forall (n : nat) (a : normal_form),
+  my_nth normal_form n work a -> Derivable ctx (nf2form a)) ->
+ (forall (a : form) (k : kripke_tree),
+  Is_Monotone_kripke_tree k ->
+  (forall b : normal_form, In b work -> forces_t k (nf2form b)) ->
+  In a ctx -> forces_t k a) ->
+ nsearch_spec_result_aux goal work DNil NNil AI_Nil ANil ctx.
+intros goal work ctx sound minimal.
+elim
+ (nsearch_aux (S (nweight_Sequent work DNil NNil AI_Nil)) goal work DNil NNil
+    AI_Nil ANil ctx).
+intros ni1 le1.
+cut (ni1 = NNil).
+intros claim.
+ rewrite claim.
+intros; assumption.
+inversion_clear le1.
+trivial.
+apply Nat.lt_succ_diag_r.
+
+unfold AI_Nil in |- *.
+unfold nf_list in |- *.
+apply regular_AVL_NIL.
+
+unfold a_ai_disj in |- *.
+intros i lookup_i bs lookup_bs.
+inversion_clear lookup_i.
+
+unfold a_goal_disj in |- *.
+intros lookup_goal.
+inversion_clear lookup_goal.
+
+unfold deco_sound in |- *.
+intros k i0 i1 b in_k.
+inversion_clear in_k.
+
+unfold nsound in |- *.
+intros a in_ngamma.
+elim in_ngamma; clear in_ngamma a.
+
+intros n a nth.
+apply sound with n; assumption.
+
+intros n i j nth; elimtype False; inversion_clear nth.
+intros n x nth; elimtype False; inversion_clear nth.
+intros i b n bs lookup_i nth; elimtype False; inversion_clear lookup_i.
+intros i lookup; elimtype False; inversion_clear lookup.
+
+unfold nminimal in |- *.
+intros a k k_is_mon k_forces_gamma in_a.
+apply minimal; try assumption.
+intros b in_b.
+elim (in_nth normal_form b work in_b).
+intros n nth.
+apply k_forces_gamma.
+apply In_Work with n; assumption.
+Qed.
+*)
+
+End NSearch.
+
+From Coq Require Extraction ExtrOcamlBasic ExtrOcamlNatInt.
+
+Set Extraction Flag 522.
+Extract Inlined Constant negb => "not".
+Extract Inlined Constant idP => "".
+Extract Inlined Constant eqn => "equal".  (* ints! *)
+Extract Inlined Constant size => "length".
+Extract Inductive reflect => bool [ true false ].
+Extract Inductive alt_spec => bool [ true false ].
+Extract Inductive eq_xor_neq => bool [ true false ].
+Extract Inductive leq_xor_gtn => bool [ true false ].
+Extract Inductive ltn_xor_geq => bool [ true false ].
+
+Extraction "ext.ml" nsearch_aux.
